---
title: "DATA 605 - Assignment 3, Problem Set 2"
author: "Amber Ferger"
date: "2/10/2020"
output: html_document
---

# Problem Set 2  
**Compute the eigenvalues and eigenvectors of the matrix A. You'll need to show your work. You'll need to write out the characteristic polynomial and show your solution.**  

$$
A = \left[\begin{array}{cc} 
1 & 2 & 3  \\
0 & 4 & 5 \\
0 & 0 & 6 
\end{array}\right]
$$ 

**Characteristic Equation:**  
$$P_{A}(x) = det(A-xI_{3})$$
$$=\left|\begin{array}{cc} 
1-x & 2 & 3  \\
0 & 4-x & 5 \\
0 & 0 & 6-x 
\end{array}\right|$$

$$=(1-x)\left|\begin{array}{cc} 
4-x & 5 \\
0 & 6-x 
\end{array}\right| - 
2\left|\begin{array}{cc} 
0 & 5 \\
0 & 6-x 
\end{array}\right| +
3\left|\begin{array}{cc} 
0 & 4-x \\
0 & 0
\end{array}\right|$$

$$= (1-x)[(4-x)(6-x)-0]-2[0]+3[0]$$
$$= (1-x)(x^2-10x+24)$$
$$= -x^3 +11x^2-34x +24$$
$$= x^3 -11x^2+34x -24$$

**Eigenvalues:**  
To find the eigenvaules of this characteristic equation, we can use the last term in our characteristic equation. The factors of 24 are: 1, 2, 3, 4, 6, 8, 12, and 24. 

**x = 1 is a solution: **
$$1^3 -11(1)^2+34(1) -24 = 0$$
$$0 = 0$$

**x = 4 is a solution: **

$$4^3 -11(4)^2+34(4) -24 = 0$$
$$0 = 0$$
**x = 6 is a solution: **  
$$6^3 -11(6)^2+34(6) -24 = 0$$
$$0 = 0$$


These 3 numbers multiply to 24 and add to 11 (our second term in the characteristic equation), so this further confirms our findings.  


**Our final eigenvalues are: **
$$\lambda_1 = 1$$
$$\lambda_2 = 4$$
$$\lambda_3 = 6$$


**Eigenvectors: ** 

$\lambda_1 = 1$

$$(A-\lambda_1I_n)x = 0 $$

$$(\left[\begin{array}{cc} 
1 & 2 & 3\\
0 & 4 & 5\\
0 & 0 & 6 \\
\end{array}\right] -
\left[\begin{array}{cc} 
1 & 0 & 0\\
0 & 1 & 0\\
0 & 0 & 1\\
\end{array}\right])(
\left[\begin{array}{cc} 
x_1 \\
x_2 \\
x_3
\end{array}\right]) = 
\left[\begin{array}{cc} 
0 \\
0 \\
0
\end{array}\right]$$

$$\left[\begin{array}{cc} 
0 & 2 & 3\\
0 & 3 & 5\\
0 & 0 & 5 \\
\end{array}\right] 
\left[\begin{array}{cc} 
x_1 \\
x_2 \\
x_3
\end{array}\right] = 
\left[\begin{array}{cc} 
0 \\
0 \\
0
\end{array}\right]$$

$$R_2 = R_2-R_3: \left[\begin{array}{cc} 0 & 2 & 3\\
0 & 3 & 0\\
0 & 0 & 5 \\
\end{array}\right] 
\left[\begin{array}{cc} 
x_1 \\
x_2 \\
x_3
\end{array}\right] = 
\left[\begin{array}{cc} 
0 \\
0 \\
0
\end{array}\right]$$

$$R_2 = \frac{1}{3}R_2: \left[\begin{array}{cc} 
0 & 2 & 3\\
0 & 1 & 0\\
0 & 0 & 5 \\
\end{array}\right] 
\left[\begin{array}{cc} 
x_1 \\
x_2 \\
x_3
\end{array}\right] = 
\left[\begin{array}{cc} 
0 \\
0 \\
0
\end{array}\right]$$

$$R_1 = R_1-2R_2: \left[\begin{array}{cc} 
0 & 0 & 3\\
0 & 1 & 0\\
0 & 0 & 5 \\
\end{array}\right] 
\left[\begin{array}{cc} 
x_1 \\
x_2 \\
x_3
\end{array}\right] = 
\left[\begin{array}{cc} 
0 \\
0 \\
0
\end{array}\right]$$

$$R_1 = \frac{1}{3}R_1: \left[\begin{array}{cc} 
0 & 0 & 1\\
0 & 1 & 0\\
0 & 0 & 5 \\
\end{array}\right] 
\left[\begin{array}{cc} 
x_1 \\
x_2 \\
x_3
\end{array}\right] = 
\left[\begin{array}{cc} 
0 \\
0 \\
0
\end{array}\right]$$

$$R_3 = R_3-5R_1: \left[\begin{array}{cc} 
0 & 0 & 1\\
0 & 1 & 0\\
0 & 0 & 0 \\
\end{array}\right] 
\left[\begin{array}{cc} 
x_1 \\
x_2 \\
x_3
\end{array}\right] = 
\left[\begin{array}{cc} 
0 \\
0 \\
0
\end{array}\right]$$

$$E_A(1) = \{\left[\begin{array}{cc} 
1 \\
0 \\
0
\end{array}\right]\}$$



###########################
$\lambda_2 = 4$

$$(A-\lambda_2I_n)x = 0 $$

$$(\left[\begin{array}{cc} 
1 & 2 & 3\\
0 & 4 & 5\\
0 & 0 & 6 \\
\end{array}\right] -
\left[\begin{array}{cc} 
4 & 0 & 0\\
0 & 4 & 0\\
0 & 0 & 4\\
\end{array}\right])(
\left[\begin{array}{cc} 
x_1 \\
x_2 \\
x_3
\end{array}\right]) = 
\left[\begin{array}{cc} 
0 \\
0 \\
0
\end{array}\right]$$

$$\left[\begin{array}{cc} 
-3 & 2 & 3\\
0 & 0 & 5\\
0 & 0 & 2 \\
\end{array}\right] 
\left[\begin{array}{cc} 
x_1 \\
x_2 \\
x_3
\end{array}\right] = 
\left[\begin{array}{cc} 
0 \\
0 \\
0
\end{array}\right]$$

$$R_3 = \frac{1}{2}R_3: \left[\begin{array}{cc} 
-3 & 2 & 3\\
0 & 0 & 5\\
0 & 0 & 1 \\
\end{array}\right] 
\left[\begin{array}{cc} 
x_1 \\
x_2 \\
x_3
\end{array}\right] = 
\left[\begin{array}{cc} 
0 \\
0 \\
0
\end{array}\right]$$

$$R_2 = R_2-5R_3: \left[\begin{array}{cc} 
-3 & 2 & 3\\
0 & 0 & 0\\
0 & 0 & 1 \\
\end{array}\right] 
\left[\begin{array}{cc} 
x_1 \\
x_2 \\
x_3
\end{array}\right] = 
\left[\begin{array}{cc} 
0 \\
0 \\
0
\end{array}\right]$$

$$R_1 = -\frac{1}{3}R_1: \left[\begin{array}{cc} 
1 & -\frac{2}{3} & -1\\
0 & 0 & 0\\
0 & 0 & 1 \\
\end{array}\right] 
\left[\begin{array}{cc} 
x_1 \\
x_2 \\
x_3
\end{array}\right] = 
\left[\begin{array}{cc} 
0 \\
0 \\
0
\end{array}\right]$$

$$R_1 = R_1+R_3: \left[\begin{array}{cc} 
1 & -\frac{2}{3} & 0\\
0 & 0 & 0\\
0 & 0 & 1 \\
\end{array}\right] 
\left[\begin{array}{cc} 
x_1 \\
x_2 \\
x_3
\end{array}\right] = 
\left[\begin{array}{cc} 
0 \\
0 \\
0
\end{array}\right]$$

$$E_A(4) = \{\left[\begin{array}{cc} 
2 \\
3 \\
0
\end{array}\right]\}$$

###########################
$\lambda_3 = 6$

$$(A-\lambda_6I_n)x = 0 $$

$$(\left[\begin{array}{cc} 
1 & 2 & 3\\
0 & 4 & 5\\
0 & 0 & 6 \\
\end{array}\right] -
\left[\begin{array}{cc} 
6 & 0 & 0\\
0 & 6 & 0\\
0 & 0 & 6\\
\end{array}\right])(
\left[\begin{array}{cc} 
x_1 \\
x_2 \\
x_3
\end{array}\right]) = 
\left[\begin{array}{cc} 
0 \\
0 \\
0
\end{array}\right]$$

$$\left[\begin{array}{cc} 
-5 & 2 & 3\\
0 & -2 & 5\\
0 & 0 & 0 \\
\end{array}\right] 
\left[\begin{array}{cc} 
x_1 \\
x_2 \\
x_3
\end{array}\right] = 
\left[\begin{array}{cc} 
0 \\
0 \\
0
\end{array}\right]$$

$$R_1 = R_1+R_2: \left[\begin{array}{cc} 
-5 & 0 & 0\\
0 & -2 & 5\\
0 & 0 & 0 \\
\end{array}\right] 
\left[\begin{array}{cc} 
x_1 \\
x_2 \\
x_3
\end{array}\right] = 
\left[\begin{array}{cc} 
0 \\
0 \\
0
\end{array}\right]$$

$$R_1 = \frac{-1}{5}R_1, R_2 = \frac{-1}{2}R_2: \left[\begin{array}{cc} 
1 & 0 & \frac{-8}{5}\\
0 & 1 & \frac{-5}{2}\\
0 & 0 & 0 \\
\end{array}\right] 
\left[\begin{array}{cc} 
x_1 \\
x_2 \\
x_3
\end{array}\right] = 
\left[\begin{array}{cc} 
0 \\
0 \\
0
\end{array}\right]$$


$$E_A(6) = \{\left[\begin{array}{cc} 
\frac{8}{5} \\
\frac{5}{2} \\
1
\end{array}\right]\} =
\{\left[\begin{array}{cc} 
16 \\
25 \\
10
\end{array}\right]\}
$$